Notations.v
@@ -361,11 +361,11 @@ Notation "'IfE' p 'ThenE' t ; cont" :=
   (IfElseE ""%string p (k' := Bit 0) t (RetE ConstDef) (fun _ => cont)) (at level 20, t at level 0): guru_scope.
 
 Notation "'LetL' letv : k' <- le ; cont" :=
-  (LetAction (Stringify letv) (k' := k') (toAction _ le) (fun letv => cont))
+  (LetActionTree (Stringify letv) (k' := k') (toActionTree _ le) (fun letv => cont))
     (at level 20, le at level 0, letv name): guru_scope.
  
 Notation "'LetL' letv <- le ; cont" :=
-  (LetAction (Stringify letv) (toAction _ le) (fun letv => cont))
+  (LetActionTree (Stringify letv) (toActionTree _ le) (fun letv => cont))
     (at level 20, le at level 0, letv name): guru_scope.
 
 Notation ITE0 p v := (ITE p v ConstTDef) (only parsing).
